Adaptable.v
@@ -2,15 +2,13 @@
 
 (**
 In Boehm's taxonomy, adaptable means that a system can change its
-state or behavior (and maybe in the future its structure) to improve its 
-fitness for purpose. Adapable here really means self-adapting. 
+state or behavior (and maybe in the future its structure) to improve its
+fitness for purpose. Adapable here really means self-adapting.
 *)
 
-Inductive Adaptable (System: Set) (Stakeholder: Set) (Context: Set) (Phase: Set) (sys: System) 
+Inductive Adaptable (System: Set) (Stakeholder: Set) (Context: Set) (Phase: Set) (sys: System)
                       : Prop :=
   satisfiesAdaptabilityRequirement:
 (exists adaptable: System -> Stakeholder -> Context -> Phase -> Prop,
     (forall cx: Context, forall sh: Stakeholder, forall ps: Phase, adaptable sys sh cx ps)) ->
       Adaptable System Stakeholder Context Phase sys.
-
-
